a 2nd example of a user-defined effect: exceptions with intrinsic and reified extrinsic proofs

examples/dm4free/Top.ml
@@ -1,4 +1,0 @@
-let _ =
-   let _, x = NatST.incr2 () (Prims.parse_int "0") in
-   print_string ("Returned: "^ Z.to_string x)
-  
